test/JexpTest.v
@@ -1,0 +1,12 @@
+From JSON Require Import
+     Encode.
+From AsyncTest Require Import
+     Jexp.
+Import JpathNotations.
+Open Scope json_scope.
+
+Example response : IR :=
+  jobj "fields" (jobj "ETag" "foo").
+
+Goal jget_weak (this@"fields"@"ETag") response = Some (JSON__String "foo").
+Proof. reflexivity. Qed.
